put the new rewrite rule in its own pass

src/Rewriter/Rules.v
@@ -561,6 +561,30 @@ Definition arith_with_casts_rewrite_rulesT (adc_no_carry_to_add : bool) : list (
              ]
         ]%Z%zrange.
 
+Definition arith_with_relaxed_casts_rewrite_rulesT : list (bool * Prop)
+  := Eval cbv [myapp mymap myflatten] in
+    myflatten
+      [mymap
+         dont_do_again
+         [(forall rland rm1 rv v,
+              rland.(upper) ∈ rm1
+              -> rland.(upper) = Z.ones (Z.succ (Z.log2 rland.(upper)))
+              -> 0 = rland.(lower)
+              -> 0 = rv.(lower)
+              -> 0 <= rv.(upper)
+              -> (rv.(upper) + 1) mod (rland.(upper) + 1) = 0
+              -> cstZ rland (Z.land (cstZ rv v) (cstZ rm1 ('rland.(upper)))) = cstZ rland v)
+          ; (forall rland rm1 rv v,
+                rland.(upper) ∈ rm1
+                -> rland.(upper) = Z.ones (Z.succ (Z.log2 rland.(upper)))
+                -> 0 = rland.(lower)
+                -> 0 = rv.(lower)
+                -> 0 <= rv.(upper)
+                -> (rv.(upper) + 1) mod (rland.(upper) + 1) = 0
+                -> cstZ rland (Z.land (cstZ rm1 ('rland.(upper))) (cstZ rv v)) = cstZ rland v)
+         ]
+      ]%Z%zrange.
+
 Definition strip_literal_casts_rewrite_rulesT : list (bool * Prop)
   := [dont_do_again (forall rx x, x ∈ rx -> cstZ rx ('x) = 'x)]%Z%zrange.
 
@@ -1060,17 +1084,7 @@ Section with_bitwidth.
           [mymap dont_do_again []
            ; mymap
                do_again
-               [
-                 (* owen put this here, and he needs to remove it. *)
-                 (forall rland rm1 rv v,
-                       rland.(upper) ∈ rm1
-                       -> rland.(upper) = Z.ones (Z.succ (Z.log2 rland.(upper)))
-                       -> 0 = rland.(lower)
-                       -> 0 = rv.(lower)
-                       -> 0 <= rv.(upper)
-                       -> (rv.(upper) + 1) mod (rland.(upper) + 1) = 0
-                       -> cstZ rland (Z.land (cstZ rv v) (cstZ rm1 ('rland.(upper)))) = cstZ rland v)
-                ; (forall A B x y, @fst A B (x, y) = x)
+               [(forall A B x y, @fst A B (x, y) = x)
                 ; (forall A B x y, @snd A B (x, y) = y)
                     (** In order to avoid tautological compares, we need to deal with carry/borrows being 0 *)
                 ; (forall r0 s x y r1 r2,
